examples/stlc/verif.v
@@ -1,9 +1,8 @@
 Require Import ssreflect ssrbool ssrnat eqtype.
+Require Import String. (* I don't know why we need this.. Probably I am forgetting something *)
 Require Import Arith List Omega QuickChick.
 Require Import lambda.
 Require Import Wellfounded.
-
-Close Scope N.
 
 Open Scope coq_nat.
 
